EC/old_info.ec
@@ -1,0 +1,410 @@
+lemma imp_policy_to_mem _policy _mem _policyAddr :
+  hoare[ConcreteScheme.policySpecToMem : policy = _policy /\
+                                         mem = _mem /\
+                                         addr = _policyAddr /\
+                                         policyFitsW64 _policy
+         ==> 
+        policyInMem _policy res _policyAddr].
+proof.
+proc.
+seq 1 : (policy = _policy /\
+         addr = _policyAddr /\
+         policyFitsW64 _policy /\
+         EqWordInt (loadW64 mem (to_uint addr)) policy.`length).
+- wp.
+  skip.
+  move => &m /> ????????????.
+  rewrite /EqWordInt.
+  rewrite load_from_store to_uint_small.
+  by do! split.
+  move => />.   
+seq 1 : (#[/:]pre /\ EqWordInt (loadW64 mem ((to_uint addr)+8)) policy.`lowercaseMin).
+- wp.
+  skip.
+  move => &m /> ???????????????????.
+  split.
+  * rewrite (load_from_unaffected_store mem{m}
+               (to_uint addr{m})
+               0
+               8
+               (of_int%W64 policy{m}.`length)
+               (of_int%W64 policy{m}.`lowercaseMin)).
+    smt.
+    trivial.
+    by apply eqwordint_int_id.
+  * rewrite load_from_store /EqWordInt to_uint_small.
+    smt.
+    reflexivity.  
+seq 1 : (#[/:]pre /\ EqWordInt (loadW64 mem ((to_uint addr)+16)) policy.`lowercaseMax).
+- wp.
+  skip.
+  move => &m /> ????????????????????.
+  do! split.
+  * rewrite (load_from_unaffected_store mem{m}
+               (to_uint addr{m})
+               0
+               16
+               (of_int%W64 policy{m}.`length)
+               (of_int%W64 policy{m}.`lowercaseMax)).
+    smt.
+    trivial.
+    by apply eqwordint_int_id.
+  * rewrite (load_from_unaffected_store mem{m}
+               (to_uint addr{m})
+               8
+               16
+               (of_int%W64 policy{m}.`lowercaseMin)
+               (of_int%W64 policy{m}.`lowercaseMax)).
+    smt.
+    trivial.
+    by apply eqwordint_int_id.
+  * rewrite load_from_store /EqWordInt to_uint_small.
+    smt.
+    reflexivity.
+seq 1 : (#[/:]pre /\ EqWordInt (loadW64 mem ((to_uint addr)+24)) policy.`uppercaseMin).
+- wp.
+  skip.
+  move => &m /> ?????????????????????.
+  do! split.
+  * rewrite (load_from_unaffected_store mem{m}
+               (to_uint addr{m})
+               0
+               24
+               (of_int%W64 policy{m}.`length)
+               (of_int%W64 policy{m}.`uppercaseMin)).
+    smt.
+    trivial.
+    by apply eqwordint_int_id.
+  * rewrite (load_from_unaffected_store mem{m}
+               (to_uint addr{m})
+               8
+               24
+               (of_int%W64 policy{m}.`lowercaseMin)
+               (of_int%W64 policy{m}.`uppercaseMin)).
+    smt.
+    trivial.
+    by apply eqwordint_int_id.
+  * rewrite (load_from_unaffected_store mem{m}
+               (to_uint addr{m})
+               16
+               24
+               (of_int%W64 policy{m}.`lowercaseMax)
+               (of_int%W64 policy{m}.`uppercaseMin)).
+    smt.
+    trivial.
+    by apply eqwordint_int_id.
+  * rewrite load_from_store /EqWordInt to_uint_small.
+    smt.
+    reflexivity.
+seq 1 : (#[/:]pre /\ EqWordInt (loadW64 mem ((to_uint addr)+32)) policy.`uppercaseMax).
+- wp.
+  skip.
+  move => &m /> ??????????????????????.
+  do! split.
+  * rewrite (load_from_unaffected_store mem{m}
+               (to_uint addr{m})
+               0
+               32
+               (of_int%W64 policy{m}.`length)
+               (of_int%W64 policy{m}.`uppercaseMax)).
+    smt.
+    trivial.
+    by apply eqwordint_int_id.
+  * rewrite (load_from_unaffected_store mem{m}
+               (to_uint addr{m})
+               8
+               32
+               (of_int%W64 policy{m}.`lowercaseMin)
+               (of_int%W64 policy{m}.`uppercaseMax)).
+    smt.
+    trivial.
+    by apply eqwordint_int_id.
+  * rewrite (load_from_unaffected_store mem{m}
+               (to_uint addr{m})
+               16
+               32
+               (of_int%W64 policy{m}.`lowercaseMax)
+               (of_int%W64 policy{m}.`uppercaseMax)).
+    smt.
+    trivial.
+    by apply eqwordint_int_id.
+  * rewrite (load_from_unaffected_store mem{m}
+               (to_uint addr{m})
+               24
+               32
+               (of_int%W64 policy{m}.`uppercaseMin)
+               (of_int%W64 policy{m}.`uppercaseMax)).
+    smt.
+    trivial.
+    by apply eqwordint_int_id.
+  * rewrite load_from_store /EqWordInt to_uint_small.
+    smt.
+    reflexivity.
+seq 1 : (#[/:]pre /\ EqWordInt (loadW64 mem ((to_uint addr)+40)) policy.`numbersMin).
+- wp.
+  skip.
+  move => &m /> ???????????????????????.
+  do! split.
+  * rewrite (load_from_unaffected_store mem{m}
+               (to_uint addr{m})
+               0
+               40
+               (of_int%W64 policy{m}.`length)
+               (of_int%W64 policy{m}.`numbersMin)).
+    smt.
+    trivial.
+    by apply eqwordint_int_id.
+  * rewrite (load_from_unaffected_store mem{m}
+               (to_uint addr{m})
+               8
+               40
+               (of_int%W64 policy{m}.`lowercaseMin)
+               (of_int%W64 policy{m}.`numbersMin)).
+    smt.
+    trivial.
+    by apply eqwordint_int_id.
+  * rewrite (load_from_unaffected_store mem{m}
+               (to_uint addr{m})
+               16
+               40
+               (of_int%W64 policy{m}.`lowercaseMax)
+               (of_int%W64 policy{m}.`numbersMin)).
+    smt.
+    trivial.
+    by apply eqwordint_int_id.
+  * rewrite (load_from_unaffected_store mem{m}
+               (to_uint addr{m})
+               24
+               40
+               (of_int%W64 policy{m}.`uppercaseMin)
+               (of_int%W64 policy{m}.`numbersMin)).
+    smt.
+    trivial.
+    by apply eqwordint_int_id.
+  * rewrite (load_from_unaffected_store mem{m}
+               (to_uint addr{m})
+               32
+               40
+               (of_int%W64 policy{m}.`uppercaseMax)
+               (of_int%W64 policy{m}.`numbersMin)).
+    smt.
+    trivial.
+    by apply eqwordint_int_id.
+  * rewrite load_from_store /EqWordInt to_uint_small.
+    smt.
+    reflexivity.
+seq 1 : (#[/:]pre /\ EqWordInt (loadW64 mem ((to_uint addr)+48)) policy.`numbersMax).
+- wp.
+  skip.
+  move => &m /> ????????????????????????.
+  do! split.
+  * rewrite (load_from_unaffected_store mem{m}
+               (to_uint addr{m})
+               0
+               48
+               (of_int%W64 policy{m}.`length)
+               (of_int%W64 policy{m}.`numbersMax)).
+    smt.
+    trivial.
+    by apply eqwordint_int_id.
+  * rewrite (load_from_unaffected_store mem{m}
+               (to_uint addr{m})
+               8
+               48
+               (of_int%W64 policy{m}.`lowercaseMin)
+               (of_int%W64 policy{m}.`numbersMax)).
+    smt.
+    trivial.
+    by apply eqwordint_int_id.
+  * rewrite (load_from_unaffected_store mem{m}
+               (to_uint addr{m})
+               16
+               48
+               (of_int%W64 policy{m}.`lowercaseMax)
+               (of_int%W64 policy{m}.`numbersMax)).
+    smt.
+    trivial.
+    by apply eqwordint_int_id.
+  * rewrite (load_from_unaffected_store mem{m}
+               (to_uint addr{m})
+               24
+               48
+               (of_int%W64 policy{m}.`uppercaseMin)
+               (of_int%W64 policy{m}.`numbersMax)).
+    smt.
+    trivial.
+    by apply eqwordint_int_id.
+  * rewrite (load_from_unaffected_store mem{m}
+               (to_uint addr{m})
+               32
+               48
+               (of_int%W64 policy{m}.`uppercaseMax)
+               (of_int%W64 policy{m}.`numbersMax)).
+    smt.
+    trivial.
+    by apply eqwordint_int_id.
+  * rewrite (load_from_unaffected_store mem{m}
+               (to_uint addr{m})
+               40
+               48
+               (of_int%W64 policy{m}.`numbersMin)
+               (of_int%W64 policy{m}.`numbersMax)).
+    smt.
+    trivial.
+    by apply eqwordint_int_id.
+  * rewrite load_from_store /EqWordInt to_uint_small.
+    smt.
+    reflexivity.
+seq 1 : (#[/:]pre /\ EqWordInt (loadW64 mem ((to_uint addr)+56)) policy.`specialMin).
+- wp.
+  skip.
+  move => &m /> ?????????????????????????.
+  do! split.
+  * rewrite (load_from_unaffected_store mem{m}
+               (to_uint addr{m})
+               0
+               56
+               (of_int%W64 policy{m}.`length)
+               (of_int%W64 policy{m}.`specialMin)).
+    smt.
+    trivial.
+    by apply eqwordint_int_id.
+  * rewrite (load_from_unaffected_store mem{m}
+               (to_uint addr{m})
+               8
+               56
+               (of_int%W64 policy{m}.`lowercaseMin)
+               (of_int%W64 policy{m}.`specialMin)).
+    smt.
+    trivial.
+    by apply eqwordint_int_id.
+  * rewrite (load_from_unaffected_store mem{m}
+               (to_uint addr{m})
+               16
+               56
+               (of_int%W64 policy{m}.`lowercaseMax)
+               (of_int%W64 policy{m}.`specialMin)).
+    smt.
+    trivial.
+    by apply eqwordint_int_id.
+  * rewrite (load_from_unaffected_store mem{m}
+               (to_uint addr{m})
+               24
+               56
+               (of_int%W64 policy{m}.`uppercaseMin)
+               (of_int%W64 policy{m}.`specialMin)).
+    smt.
+    trivial.
+    by apply eqwordint_int_id.
+  * rewrite (load_from_unaffected_store mem{m}
+               (to_uint addr{m})
+               32
+               56
+               (of_int%W64 policy{m}.`uppercaseMax)
+               (of_int%W64 policy{m}.`specialMin)).
+    smt.
+    trivial.
+    by apply eqwordint_int_id.
+  * rewrite (load_from_unaffected_store mem{m}
+               (to_uint addr{m})
+               40
+               56
+               (of_int%W64 policy{m}.`numbersMin)
+               (of_int%W64 policy{m}.`specialMin)).
+    smt.
+    trivial.
+    by apply eqwordint_int_id.
+  * rewrite (load_from_unaffected_store mem{m}
+               (to_uint addr{m})
+               48
+               56
+               (of_int%W64 policy{m}.`numbersMax)
+               (of_int%W64 policy{m}.`specialMin)).
+    smt.
+    trivial.
+    by apply eqwordint_int_id.
+  * rewrite load_from_store /EqWordInt to_uint_small.
+    smt.
+    reflexivity.
+seq 1 : (#[/:]pre /\ EqWordInt (loadW64 mem ((to_uint addr)+64)) policy.`specialMax).
+- wp.
+  skip.
+  move => &m /> ??????????????????????????.
+  do! split.
+  * rewrite (load_from_unaffected_store mem{m}
+               (to_uint addr{m})
+               0
+               64
+               (of_int%W64 policy{m}.`length)
+               (of_int%W64 policy{m}.`specialMax)).
+    smt.
+    trivial.
+    by apply eqwordint_int_id.
+  * rewrite (load_from_unaffected_store mem{m}
+               (to_uint addr{m})
+               8
+               64
+               (of_int%W64 policy{m}.`lowercaseMin)
+               (of_int%W64 policy{m}.`specialMax)).
+    smt.
+    trivial.
+    by apply eqwordint_int_id.
+  * rewrite (load_from_unaffected_store mem{m}
+               (to_uint addr{m})
+               16
+               64
+               (of_int%W64 policy{m}.`lowercaseMax)
+               (of_int%W64 policy{m}.`specialMax)).
+    smt.
+    trivial.
+    by apply eqwordint_int_id.
+  * rewrite (load_from_unaffected_store mem{m}
+               (to_uint addr{m})
+               24
+               64
+               (of_int%W64 policy{m}.`uppercaseMin)
+               (of_int%W64 policy{m}.`specialMax)).
+    smt.
+    trivial.
+    by apply eqwordint_int_id.
+  * rewrite (load_from_unaffected_store mem{m}
+               (to_uint addr{m})
+               32
+               64
+               (of_int%W64 policy{m}.`uppercaseMax)
+               (of_int%W64 policy{m}.`specialMax)).
+    smt.
+    trivial.
+    by apply eqwordint_int_id.
+  * rewrite (load_from_unaffected_store mem{m}
+               (to_uint addr{m})
+               40
+               64
+               (of_int%W64 policy{m}.`numbersMin)
+               (of_int%W64 policy{m}.`specialMax)).
+    smt.
+    trivial.
+    by apply eqwordint_int_id.
+  * rewrite (load_from_unaffected_store mem{m}
+               (to_uint addr{m})
+               48
+               64
+               (of_int%W64 policy{m}.`numbersMax)
+               (of_int%W64 policy{m}.`specialMax)).
+    smt.
+    trivial.
+    by apply eqwordint_int_id.
+  * rewrite (load_from_unaffected_store mem{m}
+               (to_uint addr{m})
+               56
+               64
+               (of_int%W64 policy{m}.`specialMin)
+               (of_int%W64 policy{m}.`specialMax)).
+    smt.
+    trivial.
+    by apply eqwordint_int_id.
+  * rewrite load_from_store /EqWordInt to_uint_small.
+    smt.
+    reflexivity.
+by skip.
+qed.
